[WTF?] what in the hell, why do they not have a collection of lemmas about the exec_* relations?

backend/SCEV.v
@@ -8,8 +8,13 @@ Require Import Integers.
 Require Import Maps.
 
 Definition nat_to_int (n: nat): int := (Int.repr (Z.of_nat n)).
-Definition Z_to_int (z: Z): int := (Int.repr z).
+Definition z_to_int (z: Z): int := (Int.repr z).
 Definition z_to_val (z: Z) : val := Vint (Int.repr z).
+
+Hint Unfold z_to_val.
+Hint Unfold z_to_int.
+Hint Transparent z_to_val.
+Hint Transparent z_to_int.
 
 (* scev for identifier "i" that starts with first val and recurrences with val *)
 Inductive scev: Type :=
@@ -32,7 +37,7 @@ Definition oned_loop (n: nat) (ivname: ident) (inner_stmt: Cminor.stmt): Cminor.
 Sloop (
     Sblock (
         Cminor.Sseq (Sifthenelse (Ebinop
-                                    (Ocmp  Clt)
+                                    (Ocmp Clt)
                                     (Evar ivname)
                                     (Econst (Ointconst (nat_to_int n))))
                                  (Sskip)
@@ -71,7 +76,174 @@ Lemma iv_init_sets_iv_value: forall (ivname: ident)
     exec_stmt ge f sp e m
               (iv_init ivname iv_init_val) E0
               e' m' Out_normal -> e' ! ivname = Some (z_to_val iv_init_val).
-Abort.
+  intros until ge.
+  intros exec.
+  inversion exec.
+  subst.
+  rewrite PTree.gss.
+  inversion_clear H4.
+  subst.
+  inversion_clear H.
+  auto.
+Qed.
+
+Lemma exec_stmt_is_function:
+  forall (m m' m'' e e' e'': env) (f: function) (sp: val) (ge: genv) (tr: trace) (o: outcome),
+  forall (s: Cminor.stmt),
+    exec_stmt ge f sp e m
+              s tr e' m' o ->
+    exec_stmt ge f sp e  m
+              s tr e'' m'' o ->
+    e' = e'' /\ m' = m''.
+
+Lemma if_cond_with_failing_branch_will_return_else:
+  forall (cond: expr) (sthen selse: Cminor.stmt),
+  forall (m m': mem) (e e': env) (f: function) (sp: val) (ge: genv) (tr: trace) (o: outcome),
+    eval_expr ge sp e m cond Vfalse ->
+    exec_stmt ge f sp e m (selse) tr e' m' o ->
+    exec_stmt ge f sp e m
+              (Cminor.Sifthenelse cond sthen selse) tr e' m' o.
+  intros until o.
+  intros exprval.
+  intros elseval.
+  assert(forall mif eif, exec_stmt ge f sp e m (Sifthenelse cond sthen selse) tr eif mif o ->
+                    eif = e' /\ mif = m').
+  intros.
+  inversion H.
+  subst.
+
+  inversion exprval.
+  subst.
+  rename H13 into ite_bool.
+  inversion H7.
+  subst.
+  rewrite H2 in H0.
+  inversion H0. subst.
+  inversion H12.
+  assert (b = false).
+  rewrite <- H1.
+  unfold negb.
+  rewrite Int.eq_true.
+  reflexivity.
+  rewrite H4 in *.
+  split.
+  
+    
+
+
+Lemma oned_loop_with_iv_gt_ub_will_not_execute:
+  forall (n: nat) (ivname: ident) (innerstmt: Cminor.stmt),
+  forall (m m': mem) (e e': env) (f: function) (sp: val) (ge: genv),
+  forall (iv_cur_z: Z),
+    e ! ivname = Some (z_to_val iv_cur_z) ->
+    Int.lt (z_to_int iv_cur_z) (nat_to_int n) = false ->
+    exec_stmt ge f sp e m
+              (oned_loop n ivname innerstmt) E0
+              e' m' (Out_exit 1) -> e = e' /\ m = m'.
+  intros until iv_cur_z.
+  intros e_at_ivname_is_iv_cur_z.
+  intros iv_cur_z_gt_n.
+  intros exec.
+  inversion exec.
+  subst.
+  
+  rename H0 into eval_sblock.
+  rename H1 into eval_sloop.
+  inversion eval_sblock. subst.
+  rename H9 into eval_sseq.
+  inversion eval_sseq.
+  subst.
+  rename H1 into exec_if.
+  rename H8 into exec_inner.
+  inversion exec_if.
+  subst.
+  rename H14 into exec_if_bool.
+  rename H8 into eval_cond.
+  inversion eval_cond.
+  subst.
+  rename H2 into eval_iv.
+  rename H5 into eval_n.
+  rename H7 into eval_cmp.
+  inversion eval_iv.
+  subst.
+  rewrite e_at_ivname_is_iv_cur_z in H0.
+  inversion H0.
+  rewrite <- H1 in *.
+  clear H1. clear H0.
+  inversion eval_cmp.
+
+  inversion eval_n.
+  subst.
+  rename H1 into eval_constant_n.
+  inversion eval_constant_n.
+  rename H0 into v2_value.
+  subst.
+  subst.
+
+
+  assert (b = false) as b_eq_false.
+  inversion eval_cond.
+  subst.
+  inversion H13.
+  subst.
+  unfold Val.cmp in H0.
+  unfold Val.of_optbool in H0.
+  unfold Val.cmp_bool in H0.
+  simpl in H0.
+  simpl in iv_cur_z_gt_n.
+  unfold z_to_int in iv_cur_z_gt_n.
+  rewrite iv_cur_z_gt_n in H0.
+  inversion H0.
+  auto.
+  rewrite b_eq_false in *.
+  inversion exec_if_bool.
+  subst.
+  rewrite <- H4 in H12.
+  inversion H7.
+  subst.
+  rename H7 into exec_ite.
+  rename H16 into exec_ite_b.
+  rename H9 into exec_binop.
+  inversion exec_binop.
+  subst.
+  inversion H2.
+  subst.
+  rewrite  e_at_ivname_is_iv_cur_z in  H0.
+  inversion H0.
+  rewrite <- H1 in *.
+  clear H0 H1.
+  inversion H5.
+  subst.
+  inversion H0.
+  unfold nat_to_int in H1.
+  rewrite <- H1 in *.
+  clear H1.
+  clear H0.
+  inversion H7.
+  unfold Val.cmp in H0. simpl in H0.
+  unfold z_to_int,nat_to_int in iv_cur_z_gt_n.
+  rewrite iv_cur_z_gt_n in H0.
+  rewrite <- H0 in *.
+  inversion H15.
+  assert (b = false).
+  rewrite <- H3. auto.
+  clear H3.
+  subst.
+  inversion exec_ite_b.
+  subst.
+  inversion eval_sloop.
+  subst.
+
+  
+
+
+
+  
+                              
+    
+
+
+Lemma 
 
 
 
